@prefix rbt: <https://riverbench.github.io/schema/theme#> .
@prefix skos: <http://www.w3.org/2004/02/skos/core#> .

rbt:conceptScheme a skos:ConceptScheme ;
    skos:prefLabel "RiverBench topic scheme"@en ;
    skos:definition "Collection of topic concepts used to annotate RiverBench datasets."@en ;
    skos:hasTopConcept rbt:rootConcept .
    
rbt:rootConcept a skos:Concept ;  
    skos:prefLabel "Root concept"@en .

rbt:temporal a skos:Concept ;
    skos:prefLabel "Temporal"@en ;
    skos:definition "Datasets with temporal information."@en ;
    skos:broader rbt:rootConcept .

rbt:spatial a skos:Concept ;
    skos:prefLabel "Spatial"@en ;
    skos:definition "Datasets with spatial information."@en ;
    skos:broader rbt:rootConcept .

rbt:statistical a skos:Concept ;
    skos:prefLabel "Statistical"@en ;
    skos:definition "Datasets with statistical information."@en ;
    skos:broader rbt:rootConcept .

rbt:sensorData a skos:Concept ;
    skos:prefLabel "Sensor data"@en ;
    skos:definition "Datasets with data from sensors, sensor networks, IoT devices, etc."@en ;
    skos:broader rbt:rootConcept .

rbt:abstract a skos:Concept ;
    skos:prefLabel "Abstract data"@en ;
    skos:definition "Datasets with abstract information (unrelated to the real world)."@en ;
    skos:broader rbt:rootConcept .
